Matching mains
Because of the relaxed connection between a program's interface and the
presence in it of a main procedure (only at the Intermediate level; in
the Source this connection is stronger), we need to state explicitly
what it means for two programs to be "mains-compatible": that is, one if
the programs has a main iff the other does.

This condition needs to be added to the standard equality of interfaces
to complete the proof of Intermediate.interface_preserves_closedness_r:
if we replace a program inside a link with another program, the
closedness of the linking is preserved if the replacement program is
sufficiently like its predecessor. Because we are requiring more than
equality of interfaces, the name is now a bit of a misnomer.

Intermediate/Machine.v
@@ -285,6 +285,9 @@ Proof.
     intuition.
 Qed.
 
+Definition matching_mains (prog1 prog2 : program) : Prop :=
+  prog_main prog1 = None <-> prog_main prog2 = None.
+
 Definition program_link (p1 p2: program): program :=
   {| prog_interface := unionm (prog_interface p1) (prog_interface p2);
      prog_procedures := unionm (prog_procedures p1) (prog_procedures p2);
@@ -836,6 +839,9 @@ Proof.
   apply prepare_procedures_initial_memory_aux_after_linking; assumption.
 Qed.
 
+(* RB: Slight "misnomer" because of the presence of matching_mains.
+   Closely connected to linkable, but not exactly the same at this
+   level. Is there a benefit to combining these two in a definition? *)
 Lemma interface_preserves_closedness_r :
   forall p1 p2 p2',
     well_formed_program p1 ->
@@ -844,12 +850,13 @@ Lemma interface_preserves_closedness_r :
     linkable (prog_interface p1) (prog_interface p2) ->
     closed_program (program_link p1 p2) ->
     linkable_mains p1 p2 ->
+    matching_mains p2 p2' ->
     closed_program (program_link p1 p2').
 Proof.
   intros p1 p2 p2'
          Hwf1 Hwf2' Hsame_int Hlinkable
          [Hclosed [mainP [main_procs [Hmain [Hprocs Hin]]]]]
-         Hlinkable_mains.
+         Hlinkable_mains Hmatching_mains.
   constructor.
   - simpl in Hclosed.
     rewrite Hsame_int in Hclosed.
@@ -881,7 +888,9 @@ Proof.
       * assumption.
     + (* main is in p2'. *)
       destruct (prog_main p2') as [main2' |] eqn:Hmain2';
-        last admit.
+        last (apply Hmatching_mains in Hmain2';
+              rewrite Hmain2' in Hmain2;
+              inversion Hmain2).
       (* Likewise main_procs (used only in second sub-goal). *)
       destruct (wfprog_main_existence Hwf2' Hmain2')
         as [main_procs2' [Hmain_procs2' Hin2']].
@@ -901,7 +910,7 @@ Proof.
       rewrite Hmain1 in Hmain.
       rewrite Hmain2 in Hmain.
       discriminate.
-Admitted.
+Qed.
 
 Lemma closed_program_link_sym p1 p2 :
   well_formed_program p1 ->
